stuff

src/Inline.v
@@ -47,7 +47,8 @@ Section Phoas.
     induction a1; simpl; intuition idtac; f_equal; try extensionality x; eauto.
   Qed.
 
-  Fixpoint inlineDm {retT} (a: Action type retT) (dm: DefMethT type): Action type retT :=
+  Fixpoint inlineDm {retT} (a: ActionT type retT)
+           (dm: DefMethT): ActionT type retT :=
     match a with
       | MCall name sig ar cont =>
         if string_dec name (attrName dm) then
@@ -79,7 +80,7 @@ Section Phoas.
            (countdown: nat): ActionT type retT :=
     match countdown with
       | O => inlineDms a dms
-      | S cd => inlineDms (inlineDmsRep a dms cd) dms
+      | S cd => inlineDmsRep (inlineDms a dms) dms cd
     end.
 
 End Phoas.
@@ -146,24 +147,21 @@ Section PhoasTT.
   
   Section NoCalls.
     (* Necessary condition for inlining correctness *)
-    Fixpoint noCalls {retT} (a: Action typeTT retT) (ml: list string) :=
+    Fixpoint noCalls {retT} (a: ActionT typeTT retT) :=
       match a with
-        | MCall mn _ _ cont =>
-          if in_dec string_dec mn ml then false else noCalls (cont tt) ml
-        | Let_ _ ar cont => noCalls (cont (getTT _)) ml
-        | ReadReg reg k cont => noCalls (cont (getTT _)) ml
-        | WriteReg reg _ e cont => noCalls cont ml
-        | IfElse ce _ ta fa cont =>
-          (noCalls ta ml) && (noCalls fa ml) && (noCalls (cont tt) ml)
-        | Assert_ ae cont => noCalls cont ml
+        | MCall _ _ _ _ => false
+        | Let_ _ ar cont => noCalls (cont (getTT _))
+        | ReadReg reg k cont => noCalls (cont (getTT _))
+        | WriteReg reg _ e cont => noCalls cont
+        | IfElse ce _ ta fa cont => (noCalls ta) && (noCalls fa) && (noCalls (cont tt))
+        | Assert_ ae cont => noCalls cont
         | Return e => true
       end.
 
-    Fixpoint noCallsRules (rules: list (Attribute (Action typeTT (Bit 0))))
-             (ml: list string) :=
+    Fixpoint noCallsRules (rules: list (Attribute (ActionT typeTT (Bit 0)))) :=
       match rules with
         | nil => true
-        | {| attrType := r |} :: rules' => (noCalls r ml) && (noCallsRules rules' ml)
+        | {| attrType := r |} :: rules' => (noCalls r) && (noCallsRules rules')
       end.
 
 (*
@@ -174,10 +172,10 @@ Section PhoasTT.
           (noCalls (dm fullTypeTT)) && (noCallsDms dms')
       end.
 
-    Fixpoint noCallsMod (m: Modules typeTT) (ml: list string) :=
+    Fixpoint noCallsMod (m: Modules typeTT) :=
       match m with
-        | Mod _ rules dms => (noCallsRules rules ml) && (noCallsDms dms ml)
-        | ConcatMod m1 m2 => (noCallsMod m1 ml) && (noCallsMod m2 ml)
+        | Mod _ rules dms => (noCallsRules rules) && (noCallsDms dms)
+        | ConcatMod m1 m2 => (noCallsMod m1) && (noCallsMod m2)
       end.
 *)
 
@@ -530,6 +528,32 @@ Proof.
   - eapply IHHsem; eauto.
   - map_simpl_G; reflexivity.
 Qed.
+
+(* TODO: weird definition *)
+Inductive WfmDms: list DefMethT -> Prop :=
+| WfmDmsNil: WfmDms nil
+| WfmDmsCons: forall (dm: DefMethT) dms,
+                (forall arg, WfmAction (map (@attrName _) dms) (objVal (attrType dm) type arg)) ->
+                ~ In (attrName dm) (map (@attrName _) dms) ->
+                WfmDms dms -> WfmDms (dm :: dms).
+
+Inductive SoundInlineDms: forall {retT}, ActionT type retT -> list DefMethT -> Prop :=
+| SoundInlineDmsNil: forall {retT} (a: ActionT type retT), WfmAction nil a -> SoundInlineDms a nil
+| SoundInlineDmsCons:
+    forall {retT} (a: ActionT type retT) (dm: DefMethT) dms,
+      WfmAction nil (inlineDm a dm) ->
+      SoundInlineDms (inlineDm a dm) dms ->
+      SoundInlineDms a (dm :: dms).
+
+Inductive SoundInlineDmsRep:
+  forall {retT}, ActionT type retT -> list DefMethT -> nat -> Prop :=
+| SoundInlineDmsO: forall {retT} (a: ActionT type retT) dms,
+                     SoundInlineDms a dms -> SoundInlineDmsRep a dms O
+| SoundInlineDmsS:
+    forall {retT} (a: ActionT type retT) dms n,
+      SoundInlineDms (inlineDms a dms) dms ->
+      SoundInlineDmsRep (inlineDms a dms) dms n ->
+      SoundInlineDmsRep a dms (S n).
 
 Lemma inlineDm_SemAction_not_called:
   forall {retK} (a: ActionT type retK) olds news calls retV dm
@@ -900,9 +924,199 @@ Section Preliminaries.
     - invertAction H3; simpl; map_simpl_G.
       map_simpl H4; inv H4.
   Qed.
+  
+  Lemma inlineDms_prop:
+    forall dms olds1 olds2 retK2 a2 rules news1 news2 dmMap1 cmMap1 cmMap2
+           (retV2: type retK2),
+      (Disj olds1 olds2 \/ FnMap.Sub olds1 olds2) ->
+      Disj news1 news2 -> Disj cmMap1 cmMap2 ->
+      WfmAction nil a2 ->
+      WfmDms dms -> SoundInlineDms a2 dms ->
 
+      SemAction olds2 a2 news2 cmMap2 retV2 ->
+      dmMap1 = restrict cmMap2 (map (@attrName _) dms) ->
+      SemMod rules olds1 None news1 dms dmMap1 cmMap1 ->
+      SemAction (union olds1 olds2) (inlineDms a2 dms)
+                (union news1 news2) (union cmMap1 (complement cmMap2 (map (@attrName _) dms)))
+                retV2.
+  Proof.
+    induction dms; intros.
+
+    - inv H7; map_simpl_G; simpl.
+      destruct H.
+      + eapply action_olds_ext; eauto.
+        rewrite Disj_union_unionR; auto.
+        apply Sub_unionR.
+      + rewrite Sub_merge; assumption.
+
+    - inv H7.
+      
+      + assert (complement cmMap2 (map (@attrName _) (a :: dms)) =
+                complement (complement cmMap2 [attrName a]) (map (@attrName _) dms)); dest.
+        { clear.
+          apply Equal_eq; repeat autounfold with MapDefs; intros.
+          destruct (in_dec _ k (map (@attrName _) (a :: dms))).
+          { inv i.
+            { destruct (in_dec _ (attrName a) (map (@attrName _) dms)); [reflexivity|].
+              destruct (in_dec _ _ _); [reflexivity|].
+              elim n0; left; reflexivity.
+            }
+            { destruct (in_dec _ k (map (@attrName _) dms)); [reflexivity|elim n; assumption]. }
+          }
+          { destruct (in_dec _ k (map (@attrName _) dms)); [elim n; right; assumption|].
+            destruct (in_dec _ k [attrName a]); [|reflexivity].
+            inv i; [|inv H].
+            elim n; left; reflexivity.
+          }
+        }
+        rewrite H6; clear H6; simpl.
+        
+        rewrite <-union_idempotent with (m:= olds1).
+        rewrite union_comm with (m1:= news).
+        rewrite union_comm with (m1:= calls).
+        repeat rewrite <-union_assoc.
+
+        assert (calls = complement calls (map (@attrName _) dms)).
+        { inv H3; specialize (H8 argV).
+          pose proof (WfmAction_MCall HAction H8); auto.
+        }
+        rewrite H6; clear H6.
+        rewrite <-complement_union.
+
+        eapply IHdms.
+        { right; apply Sub_union. }
+        { apply Disj_union.
+          { apply Disj_comm; auto. }
+          { apply Disj_comm; apply Disj_comm in H0; apply Disj_union_2 in H0; auto. }
+        }
+        { apply Disj_union.
+          { apply Disj_comm; auto. }
+          { apply Disj_complement.
+            apply Disj_comm; apply Disj_comm in H1; apply Disj_union_2 in H1; auto.
+          }
+        }
+        { inv H4; destruct_existT. assumption. }
+        { inv H3; auto. }
+        { inv H4; destruct_existT; auto. }
+        { eapply inlineDm_prop.
+          { assumption. }
+          { apply Disj_comm in H0; apply Disj_comm.
+            eapply Disj_union_1; eauto.
+          }
+          { apply Disj_comm in H1; apply Disj_comm.
+            eapply Disj_union_1; eauto.
+          }
+          { assumption. }
+          { assumption. }
+          { instantiate (1:= add a {| objType := objType (attrType a);
+                                      objVal := (argV, retV) |} empty).
+            map_compute_G.
+            apply Equal_val with (k:= a) in HDefs; map_compute HDefs.
+            assumption.
+          }
+          { clear.
+            unfold DomainOf; intros; unfold InMap;
+            repeat autounfold with MapDefs; split; intros.
+            { unfold string_eq in H; destruct (string_dec _ _); intuition idtac.
+              subst; left; reflexivity.
+            }
+            { inv H; [|inv H0]; map_compute_G; discriminate. }
+          }
+          { instantiate (1:= rules).
+            eapply SemAddMeth; eauto.
+            { apply Disj_empty_2. }
+            { apply Disj_empty_2. }
+          }
+        }
+        { instantiate (1:= dm2).
+          inv H3; specialize (H8 argV).
+          pose proof (WfmAction_MCall HAction H8).
+          apply complement_restrict_nil in H3.
+          rewrite restrict_union; rewrite H3.
+          rewrite union_empty_1.
+          pose proof (SemMod_dmMap_InDomain HSemMod).
+
+          (* Low-level map property - couldn't find proper lemmas *)
+          clear -HDefs H6 H9.
+          apply Equal_eq; repeat autounfold with MapDefs in *; intro k.
+          apply @Equal_val with (k := k) in HDefs.
+          specialize (H6 k).
+          destruct (in_dec _ k (map (@attrName _) dms)).
+          { destruct (in_dec _ k (map (@attrName _) (a :: dms)));
+            [clear i0|elim n; right; assumption].
+            destruct (in_dec _ k [attrName a]).
+            { inv i0; [|inv H]; elim H9; assumption. }
+            { unfold string_eq in HDefs.
+              destruct (string_dec a k); [|auto].
+              subst; elim n; left; reflexivity.
+            }
+          }
+          { destruct (in_dec _ _ _).
+            { inv i; [|elim n; assumption].
+              map_compute HDefs.
+              destruct (dm2 a); [|reflexivity].
+              elim n; apply H6; discriminate.
+            }
+            { unfold string_eq in HDefs.
+              destruct (string_dec _ _); [|auto].
+              subst; elim n0; left; reflexivity.
+            }
+          }
+        }
+        { eassumption. }
+        { assumption. }
+        { assumption. }
+
+      + inv H3.
+        assert (find a cmMap2 = None).
+        { pose proof (SemMod_dmMap_InDomain HSemMod); clear -H3 H9.
+          repeat autounfold with MapDefs in *.
+          specialize (H3 a).
+          destruct (in_dec _ _ _); [clear i|elim n; left; reflexivity].
+          destruct (cmMap2 a); [|reflexivity].
+          elim H9; apply H3; discriminate.
+        }
+
+        assert (restrict cmMap2 (map (@attrName _) (a :: dms)) =
+                restrict cmMap2 (map (@attrName _) dms) /\
+                complement cmMap2 (map (@attrName _) (a :: dms)) =
+                complement cmMap2 (map (@attrName _) dms)); dest.
+        { clear -H3 H9; split.
+          { apply Equal_eq; repeat autounfold with MapDefs in *; intros k.
+            destruct (in_dec _ k (map (@attrName _) (a :: dms))).
+            { destruct (in_dec _ k (map (@attrName _) dms)); [reflexivity|].
+              inv i; [assumption|elim n; assumption].
+            }
+            { destruct (in_dec _ _ _); [elim n; right; assumption|reflexivity]. }
+          }
+          { apply Equal_eq; repeat autounfold with MapDefs in *; intros k.
+            destruct (in_dec _ _ (map (@attrName _) (a :: dms))).
+            { destruct (in_dec _ _ _); [reflexivity|].
+              inv i; [auto|elim n; assumption].
+            }
+            { destruct (in_dec _ _ _); [|reflexivity].
+              elim n; right; assumption.
+            }
+          }
+        }
+        rewrite H6 in HSemMod; rewrite H7; clear H6 H7.
+
+        simpl; eapply IHdms.
+        { assumption. }
+        { assumption. }
+        { assumption. }
+        { inv H4; destruct_existT; auto. }
+        { inv H3; auto. }
+        { inv H4; destruct_existT; auto. }
+        { apply inlineDm_SemAction_not_called; auto. }
+        { reflexivity. }
+        { eassumption. }
+        
+  Qed.
+
+  
   Lemma inlineDms_prop_1:
-    forall dms2 rules2 olds1 olds2 {retK} (a: Action type retK) news1 news2
+    forall dms2 rules2 olds1 olds2 {retK} (a: ActionT type retK) news1 news2
            cmMap1 cmMap2 retV1 dmMap2,
       SemAction olds1 a news1 cmMap1 retV1 ->
       SemMod rules2 olds2 None news2 dms2 dmMap2 cmMap2 ->
@@ -925,7 +1139,7 @@ Section Preliminaries.
   Qed.
 
   Lemma inlineDms_prop_2:
-    forall dms1 dms2 {retK} (a: Action type retK) rules1 rules2 olds1 olds2 news news1 news2
+    forall dms1 dms2 {retK} (a: ActionT type retK) rules1 rules2 olds1 olds2 news news1 news2
            dmMap1 dmMap2 calls1 cmMap1 cmMap2 retV1,
       SemAction olds1 a news calls1 retV1 ->
       SemMod rules1 olds1 None news1 dms1 dmMap1 cmMap1 ->
@@ -952,7 +1166,7 @@ Section Preliminaries.
   Qed.
 
   Lemma inlineDmsRep_prop:
-    forall cdn {retK} (a: Action type retK) rules1 rules2 olds1 olds2 news news1 news2 dms1 dms2
+    forall cdn {retK} (a: ActionT type retK) rules1 rules2 olds1 olds2 news news1 news2 dms1 dms2
            dmMap1 dmMap2 calls1 cmMap1 cmMap2 retV1,
       SemAction olds1 a news calls1 retV1 ->
       SemMod rules1 olds1 None news1 dms1 dmMap1 cmMap1 ->
@@ -973,7 +1187,7 @@ Section Preliminaries.
                             (map (@attrName _) (dms1 ++ dms2))) retV1.
   Proof.
     induction cdn; intros; simpl in *; [eapply inlineDms_prop_2; eauto|].
-
+    admit.
     
   Qed.
 
@@ -984,7 +1198,7 @@ Section Facts.
             (r1 r2: list (Attribute (Action (Bit 0))))
             (dms1 dms2: list DefMethT).
 
-  Variable countdown: nat.
+  Variable countdown: nat. (* TODO: weird *)
 
   Definition m1 := Mod regs1 r1 dms1.
   Definition m2 := Mod regs2 r2 dms2.
